verif/btrees.v
@@ -435,17 +435,20 @@ Fixpoint moveToFirst {X:Type} (n:node X) (c:cursor X) (level:nat): cursor X :=
   end.
 
 (* takes a PARTIAL cursor, n next node (pointed to by the cursor) and goes down to last key *)
-Fixpoint moveToLast {X:Type} (n:node X) (c:cursor X) (level:nat): cursor X :=
+Function moveToLast {X:Type} (n:node X) (c:cursor X) (level:nat) {measure node_depth n}: cursor X :=
   match n with
     btnode ptr0 le isLeaf First Last x =>
     match isLeaf with
     | true => (n,ip (numKeys n))::c
     | false => match (nth_node (ip(numKeys n -1)) n)  with
                | None => c      (* not possible, isLeaf is false *)
-               | Some n' => moveToFirst n' ((n,ip (numKeys n -1))::c) (level+1)
+               | Some n' => moveToLast n' ((n,ip (numKeys n -1))::c) (level+1)
                end
     end
   end.
+Proof.
+  intros. apply nth_node_decrease in teq1. auto.
+Qed.
 
 (* takes a PARTIAL cursor, n next node (pointed to by the cursor) and goes down to the key, or where it should be inserted *)
 Function moveToKey {X:Type} (n:node X) (key:key) (c:cursor X) {measure node_depth n} : cursor X :=
@@ -631,7 +634,7 @@ Definition moveToPrev {X:Type} (c:cursor X) (r:relation X) : cursor X :=
           match (nth_node i n) with
           | None => cdecr       (* impossible *)
           | Some n' =>
-            moveToLast n' cdecr (length cdecr) (* going down on the left if we had to go up *)
+            moveToLast X n' cdecr (length cdecr) (* going down on the left if we had to go up *)
           end
         end
       end
