verif/verif_movetolast.v
@@ -16,7 +16,202 @@ Require Import btrees_sep.
 Require Import btrees_spec.
 Require Import index.
 
-Lemma body_moveToLast: semax_body Vprog Gprog f_moveToFirst moveToLast_spec.
+Lemma body_moveToLast: semax_body Vprog Gprog f_moveToLast moveToLast_spec.
 Proof.
   start_function.
-Admitted.
+  destruct r as [root prel].
+  pose (r:=(root,prel)). fold r.
+  destruct n as [ptr0 le isLeaf First Last pn].
+  pose (n:=btnode val ptr0 le isLeaf First Last pn). fold n.
+  assert(CLENGTH: 0 <= Zlength c < 20).
+  { unfold partial_cursor in H. destruct H. unfold correct_depth in H3.
+    rewrite Zlength_correct. apply partial_rel_length in H. rep_omega. }
+  assert(GETVAL: pn = getval n). { unfold n. simpl. auto. }
+  assert(SUBNODE: subnode n root).
+  { unfold partial_cursor in H. destruct H.
+    simpl in H1. unfold partial_cursor_correct_rel in H.
+    destruct c as [|[n' i ] c'].
+    - simpl in H2. inversion H2. unfold n. apply sub_refl.
+    - simpl in H2. rewrite H2 in H. simpl in H. destruct H.
+      apply partial_cursor_subnode' in H. apply nth_subnode in H2.
+      apply sub_trans with (n0:=n) in H. auto. unfold n. auto. }
+  assert_PROP(isptr pn).
+  { unfold relation_rep. unfold r. apply subnode_rep in SUBNODE. rewrite SUBNODE.
+    rewrite GETVAL. Intros. entailer!. }
+  assert(ISPTR: isptr pn) by auto. clear H4.
+
+  forward_if (
+      PROP(pn<>nullval)
+      LOCAL(temp _cursor pc; temp _node pn; temp _level (Vint (Int.repr (Zlength c))))
+      SEP(relation_rep r; cursor_rep c r pc))%assert.
+  - apply denote_tc_test_eq_split. assert (SUBREP: subnode n root) by auto.
+    apply subnode_rep in SUBREP. rewrite SUBREP. rewrite GETVAL. entailer!.
+    entailer!.    
+  - forward.                    (* skip *)
+    entailer!.
+  - assert (SUBREP: subnode n root) by auto.
+    apply subnode_rep in SUBREP. unfold relation_rep. unfold r.
+    rewrite SUBREP.
+    assert_PROP(isptr (getval n)). entailer!.
+    rewrite <- GETVAL in H5. rewrite H4 in H5. simpl in H5. contradiction.
+  - forward_if (
+        (PROP (pn <> nullval; pc <> nullval)
+         LOCAL (temp _cursor pc; temp _node pn; temp _level (Vint (Int.repr (Zlength c))))
+         SEP (relation_rep r; cursor_rep c r pc))).
+    + forward. entailer!.
+    + assert_PROP(False).
+      entailer!. contradiction.
+    + forward_if ((PROP (pn <> nullval; pc <> nullval; (Zlength c) >= 0)
+     LOCAL (temp _cursor pc; temp _node pn; temp _level (Vint (Int.repr (Zlength c))))
+     SEP (relation_rep r; cursor_rep c r pc))).
+      * forward. entailer!.
+      * assert_PROP(False). entailer. omega.
+      * unfold cursor_rep.
+        Intros anc_end. Intros idx_end. unfold r.
+        forward.                (* cursor->ancestors[level]=node *)
+        forward.                (* cursor->level = level *) 
+        assert (SUBREP:subnode n root) by auto.
+        apply subnode_rep in SUBREP. unfold relation_rep. rewrite SUBREP. unfold n.
+        rewrite unfold_btnode_rep at 1. Intros ent_end.
+        forward.                (* t'2=node->isLeaf *)
+        { entailer!. destruct isLeaf; simpl; auto. }  
+        forward_if.
+{
+  - forward.                    (* t'5=node->numKeys *)
+    forward.                    (* cursor->ancestorsIdx[level]=t'5 *)
+    + gather_SEP 2 3 4 5. replace_SEP 0 (btnode_rep (btnode val ptr0 le isLeaf First Last pn)).
+      { rewrite unfold_btnode_rep. entailer!. Exists ent_end. entailer!. }
+      gather_SEP 0 3. replace_SEP 0 (btnode_rep root).
+      { rewrite unfold_btnode_rep with (n:=root). entailer!. apply wand_frame_elim'. cancel. }
+      gather_SEP 0 1 2. replace_SEP 0 (relation_rep r).
+      { entailer!. }
+      gather_SEP 1 2. replace_SEP 0 (cursor_rep (moveToLast val n c (length c)) r pc).
+      { entailer!. unfold cursor_rep.
+        Exists (sublist 1 (Zlength anc_end) anc_end). Exists (sublist 1 (Zlength idx_end) idx_end).
+        unfold r. fold n.
+        assert (Zlength ((n,ip (numKeys_le le))::c) -1 = Zlength c). { rewrite Zlength_cons. omega. }
+        rewrite moveToLast_equation. simpl.
+        rewrite H7. cancel. 
+        autorewrite with sublist. simpl. rewrite <- app_assoc. rewrite <- app_assoc.
+        rewrite upd_Znth0. rewrite upd_Znth0. cancel. }
+      forward.                  (* return *)
+      unfold r. fold n. entailer!.
+} {
+  forward.                      (* skip *)
+  forward.                      (* t'3=node->numKeys *)
+  forward.                      (* cursor->ancestorsIdx[level]=t'3-1 *)
+  { assert(Int.min_signed <= Z.of_nat (numKeys_le le) <= Int.max_signed).
+    { split. rep_omega. unfold root_wf, node_wf in H1. simpl in H1.
+      apply H1 in SUBNODE. unfold n in SUBNODE. simpl in SUBNODE. rep_omega. }
+    entailer!. }
+  -                             (* recursive call *)
+    destruct ptr0 as [ptr0n|] eqn:EQPTR0.
+    + destruct ptr0n eqn:EPTR0n.
+      { 
+      Intros.
+      forward.                    (* t'1=node->ptr0 *)
+      gather_SEP 2 3 4 5. replace_SEP 0 (btnode_rep (btnode val ptr0 le isLeaf First Last pn)).
+      { rewrite unfold_btnode_rep with (n:=btnode val ptr0 le isLeaf First Last pn).
+        entailer!. Exists ent_end. entailer!. }
+      gather_SEP 0 3. replace_SEP 0 (btnode_rep root).
+      { rewrite EQPTR0. pose (btnoderep:=btnode_rep (btnode val (Some (btnode val o l b b0 b1 v)) le isLeaf First Last pn)). fold btnoderep.
+      pose(btroot:=btnode_rep root). fold btroot.
+      entailer!. apply wand_frame_elim. }
+      gather_SEP 0 1 2. replace_SEP 0 (relation_rep r).
+      { entailer!. }
+      deadvars!. simpl.
+
+      rewrite SUBREP. rewrite unfold_btnode_rep with (n:=n) at 1. unfold n. clear ent_end.
+      Intros ent_end. simpl. fold n.
+      destruct le as [|firste le'] eqn:HLE.
+      { exfalso. subst isLeaf. unfold root_integrity in H0. apply H0 in SUBNODE.
+        unfold n in SUBNODE. simpl in SUBNODE. inv SUBNODE. }
+      assert(HZNTH: (numKeys_le le - 1 < numKeys_le le)%nat).
+      { rewrite HLE. simpl. omega. }
+      apply nth_entry_le_in_range in HZNTH.
+      destruct HZNTH as [laste HZNTH].
+      assert(KC: nth_entry (numKeys_le le - 1) n = Some laste).
+      { unfold n. rewrite <- HLE. simpl. auto. }
+      apply integrity_nth in KC. destruct KC as [k [child HLAST]]. subst laste.
+      assert (HNTH: nth_entry (numKeys_le le - 1) n = Some (keychild val k child)).
+      { unfold n. rewrite <- HLE. simpl. auto. }
+      eapply Znth_to_list with (endle := ent_end) in HZNTH.
+      assert(SUBCHILD: subnode child root).
+      { apply sub_trans with (n1:=n). eapply entry_subnode. eauto. auto. }
+      rewrite HLE in HZNTH. simpl in HZNTH.
+      rewrite Nat2Z.inj_sub in HZNTH by omega. simpl in HZNTH. rewrite Z.sub_0_r in HZNTH.
+      forward.                  (* t'2=node->entries[t'1-1]->ptr.child *)
+      { rewrite Zpos_P_of_succ_nat. rewrite Zsuccminusone.
+        entailer!. unfold root_wf, node_wf in H1. apply H1 in SUBNODE.
+        split. omega.
+        rewrite Fanout_eq in SUBNODE. unfold n in SUBNODE. simpl in SUBNODE. rep_omega. }
+      { rewrite Zpos_P_of_succ_nat. rewrite Zsuccminusone. rewrite HZNTH.
+        apply subnode_rep in SUBCHILD.
+        gather_SEP 2 3 4 5. replace_SEP 0 (btnode_rep n).
+        { entailer!. rewrite unfold_btnode_rep with (n:=n). unfold n.
+          Exists ent_end. cancel. }
+        gather_SEP 0 3. replace_SEP 0 (btnode_rep root).
+        { entailer!. apply wand_frame_elim. }
+        rewrite SUBCHILD. entailer!. }        
+      { entailer!. rewrite Zpos_P_of_succ_nat. rewrite Int.signed_repr with (z:=1) by rep_omega.
+        clear -H1 SUBNODE. unfold root_wf, node_wf in H1. simpl in H1. apply H1 in SUBNODE.
+        unfold n in SUBNODE. simpl in SUBNODE.
+        rewrite Int.signed_repr. rewrite Zsuccminusone. rep_omega.
+        rep_omega. }
+      rewrite Zpos_P_of_succ_nat. rewrite Zsuccminusone.
+      simpl le_to_list. rewrite <- app_comm_cons.
+      rewrite HZNTH.
+      gather_SEP 2 3 4 5. replace_SEP 0 (btnode_rep n).
+      { entailer!. rewrite unfold_btnode_rep with (n:=n). unfold n.
+        Exists ent_end. entailer!. }
+      gather_SEP 0 3. replace_SEP 0 (btnode_rep root).
+      { entailer!. apply wand_frame_elim. }
+      
+      forward_call(r,((n,ip(numKeys_le le -1))::c),pc,child). (* moveToLast *)      
+      * entailer!. repeat apply f_equal. rewrite Zlength_cons. omega.
+      * unfold cursor_rep. unfold r.
+        Exists (sublist 1 (Zlength anc_end) anc_end). Exists (sublist 1 (Zlength idx_end) idx_end).
+        assert (Zlength ((n,ip(numKeys_le le -1))::c) -1 = Zlength c). rewrite Zlength_cons. omega.
+        rewrite H8. change_compspecs CompSpecs. cancel.
+        autorewrite with sublist. simpl. rewrite <- app_assoc. rewrite <- app_assoc.
+        rewrite upd_Znth0. rewrite upd_Znth0. autorewrite with norm.
+        rewrite Zpos_P_of_succ_nat. rewrite Zsuccminusone. rewrite HLE.
+        simpl. rewrite Nat2Z.inj_sub by omega. simpl. rewrite Z.sub_0_r. cancel.
+        change_compspecs CompSpecs. cancel.
+      * split.
+        { unfold partial_cursor in *.
+          destruct H. split.
+          - simpl. assert(nth_node_le (numKeys_le le -1) (cons val firste le') = Some child).
+            { eapply nth_entry_child. unfold n in HNTH. simpl in HNTH. eauto. }
+            rewrite H9. split; auto.
+            unfold partial_cursor_correct.
+            destruct c as [|[n' i] c']. simpl in H2. simpl. fold n in H2. inversion H2. auto.
+            split.
+            + simpl in H. destruct (nth_node i n').
+              destruct H. auto.
+              inv H.
+            + fold n in H2. simpl in H2. auto.
+          - auto. }
+        { split.
+          - auto.
+          - split.
+            + simpl. auto.
+            + split. simpl.
+              eapply nth_entry_child. unfold n in HNTH. simpl in HNTH. eauto.
+              auto. }
+      * forward.
+        (* instantiate (Frame:=[]). *) entailer!.
+        fold r. simpl. rewrite moveToLast_equation with (c:=c).
+        simpl.
+        assert(nth_node_le (numKeys_le le' -0) (cons val firste le') = Some child).
+        { eapply nth_entry_child. unfold n in HNTH. simpl in HNTH. eauto. }
+        rewrite H7. fold n.
+        assert((S (length c)) = (length c + 1)%nat) by omega.
+        rewrite H13. cancel.
+      * auto.
+      * unfold n. simpl. rewrite H7. auto. }
+    +                           (* ptr0 has to be defined on an intern node *)
+      unfold root_integrity in H0. unfold get_root in H0. simpl in H0.
+      apply H0 in SUBNODE. unfold node_integrity in SUBNODE.
+      unfold n in SUBNODE. rewrite H7 in SUBNODE. contradiction. }
+Qed.
